acl2svn/branches/centaur/defthm.lisp
@@ -3823,11 +3823,13 @@
   thorough understanding of them before proceeding (at which time
   ~pl[extended-metafunctions]).
 
-  Metafunctions and (if supplied) hypothesis metafunctions must be executable.
-  That is, they cannot be constrained (i.e., introduced in the ~il[signature]
-  of ~ilc[encapsulate] ~il[events]), nor can they be ~il[declare]d
+  One might think that metafunctions and (if supplied) hypothesis metafunctions
+  must be executable: that is, not constrained (i.e., introduced in the
+  ~il[signature] of ~ilc[encapsulate] ~il[events]), and not ~il[declare]d
   ~c[:]~ilc[non-executable].  After all, there is no point in installing a
-  simplifier that cannot be run!
+  simplifier that cannot be run!  However, such a restriction is not enforced,
+  because one could introduce a metafunction using ~ilc[encapsulate] and then
+  use ~ilc[defattach] to attach it to an executable function; ~pl[defattach].
 
   We defer discussion of the case in which there is a hypothesis metafunction
   and for now address the case in which the other two hypotheses are present.
@@ -5730,15 +5732,6 @@ this problem.  [It contains a truly trivial edit we've made, not important.]
                  (null (f-get-global 'in-local-flg state)))
                 'illegal)
                (t 'maybe)))))
-
-(defun attachment-alist (fn wrld)
-  (let ((prop (getprop fn 'attachment nil 'current-acl2-world wrld)))
-    (and prop
-         (cond ((symbolp prop)
-                (getprop prop 'attachment nil 'current-acl2-world wrld))
-               ((eq (car prop) :attachment-disallowed)
-                prop) ; (cdr prop) follows "because", e.g., (msg "it is bad")
-               (t prop)))))
 
 (defun attached-fns (fns wrld)
   (cond ((endp fns) nil)
