acl2svn/branches/centaur/type-set-b.lisp
@@ -1133,36 +1133,32 @@
               (convert-theory-to-unordered-mapping-pairs lst wrld)))
             wrld))))
 
-; We now develop the foundations of the concept that a rune is
-; "enabled" in the current theory.  In ACL2, the user can get "into" a
-; theory with the in-theory event, which is similar in spirit to
-; in-package but selects a theory as the "current" theory.  A rune is
-; said to be "enabled" if it is a member of the runic theory
-; corresponding to the current (common) theory and is said to be
+; We now develop the foundations of the concept that a rune is "enabled" in the
+; current theory.  In ACL2, the user can get "into" a theory with the in-theory
+; event, which is similar in spirit to in-package but selects a theory as the
+; "current" theory.  A rune is said to be "enabled" if it is a member of the
+; runic theory corresponding to the current (common) theory and is said to be
 ; "disabled" otherwise.
 
 ; Historical Note about Nqthm
 
-; Nqthm had no explicit notion of the current theory.  However,
-; implicitly, nqthm contained a current theory and the events ENABLE
-; and DISABLE allowed the user to add a name to it or delete a name
-; from it.  The experimental xnqthm, mentioned elsewhere in this
-; system, introduced the notion of theories and tied them to enabling
-; and disabling, following suggestions and patches implemented by Bill
-; Bevier during the Kit proofs (and implemented in Pc-Nqthm, and
-; extended in Nqthm-1992).  The ACL2 notion of theory is much richer
-; because it allows one to compute the value of theories using
-; functions defined within the logic.  (end of note)
+; Nqthm had no explicit notion of the current theory.  However, implicitly,
+; nqthm contained a current theory and the events ENABLE and DISABLE allowed
+; the user to add a name to it or delete a name from it.  The experimental
+; xnqthm, mentioned elsewhere in this system, introduced the notion of theories
+; and tied them to enabling and disabling, following suggestions and patches
+; implemented by Bill Bevier during the Kit proofs (and implemented in
+; Pc-Nqthm, and extended in Nqthm-1992).  The ACL2 notion of theory is much
+; richer because it allows one to compute the value of theories using functions
+; defined within the logic.  (end of note)
 
-; Suppose we have a theory which has been selected as current.  This
-; may be the globally current theory, as set by the in-theory event,
-; or it may be a locally current theory, as set by the in-theory hint
-; to defthm or defun.  We must somehow process the current theory so
-; that we can quickly answer the question "is rune enabled?"  We now
-; develop the code for doing that.
+; Suppose we have a theory which has been selected as current.  This may be the
+; globally current theory, as set by the in-theory event, or it may be a
+; locally current theory, as set by the in-theory hint to defthm or defun.  We
+; must somehow process the current theory so that we can quickly answer the
+; question "is rune enabled?"  We now develop the code for doing that.
 
-; The structure defined below is used as a fast way to represent a
-; theory:
+; The structure defined below is used as a fast way to represent a theory:
 
 (defrec enabled-structure
 
@@ -1173,85 +1169,80 @@
    array-name-root . array-name-suffix)
   t)
 
-; The following invariant is maintained in all instances of this
-; structure.  Theory-array is an array1p whose array length is
-; array-length.  Furthermore array-name is a symbol of the form rootj,
-; root is the array-name-root (as a list of characters) and j is the
-; array-name-suffix.  Thus, if i is a nonnegative integer less than
-; array-length, then (acl2-aref1 array-name theory-array i) has a
-; satisfied guard.  Furthermore, important to efficiency but
-; irrelevant to correctness, it will always be the case that the von
-; Neumann array associated with array-name is in fact theory-array.
-; Thus the above expression executes quickly.  To get a new array
-; name, should one ever be needed, it suffices to increment the
-; array-name-suffix and build a name from that new value.
+; The following invariant is maintained in all instances of this structure.
+; Theory-array is an array1p whose array length is array-length.  Furthermore
+; array-name is a symbol of the form rootj, root is the array-name-root (as a
+; list of characters) and j is the array-name-suffix (which however is not
+; always used; see load-theory-into-enabled-structure).  Thus, if i is a
+; nonnegative integer less than array-length, then (acl2-aref1 array-name
+; theory-array i) has a satisfied guard.  Furthermore, important to efficiency
+; but irrelevant to correctness, it will always be the case that the von
+; Neumann array associated with array-name is in fact theory-array.  Thus the
+; above expression executes quickly.  To get a new array name, should one ever
+; be needed, it can suffice to increment the array-name-suffix and build a name
+; from that new value.  However, if we hope to use parallel evaluation in the
+; waterfall, we instead make a unique name based on each clause-id.  See
+; load-theory-into-enabled-structure.
 
-; The theory-array of an enabled-structure for a given common theory
-; is (except for the header entry) just the augmented runic theory
-; corresponding to the given common theory.  That is, the ACL2 array
-; alist we need to construct for a theory maps each array index to a
-; non-nil value.  The non-nil value we choose is in fact the
-; corresponding rune.  It would suffice, for purposes of enabling, to
-; store T in the array to signify enabledness.  By storing the rune
-; itself we make it possible to determine what runic theory is in the
-; array.  (There is no general purpose way to map from a nume to its
-; rune (short of looking through the whole world).)
+; The theory-array of an enabled-structure for a given common theory is (except
+; for the header entry) just the augmented runic theory corresponding to the
+; given common theory.  That is, the ACL2 array alist we need to construct for
+; a theory maps each array index to a non-nil value.  The non-nil value we
+; choose is in fact the corresponding rune.  It would suffice, for purposes of
+; enabling, to store T in the array to signify enabledness.  By storing the
+; rune itself we make it possible to determine what runic theory is in the
+; array.  (There is no general purpose way to map from a nume to its rune
+; (short of looking through the whole world).)
 
-; The global variable 'global-enabled-structure contains an instance
-; of the enabled-structure record in which the array-name is
-; ENABLED-ARRAY-0, array-name-root is the list of characters in
-; "ENABLED-ARRAY-" and the array-name-suffix is 0.  A rune with
-; nume n is (globally) enabled in the current world iff either n is
-; greater than the index-of-last-enabling or array[n] is non-nil.
-; This is just the computation done by enabled-numep, below.
+; The global variable 'global-enabled-structure contains an instance of the
+; enabled-structure record in which the array-name is ENABLED-ARRAY-0,
+; array-name-root is the list of characters in "ENABLED-ARRAY-" and the
+; array-name-suffix is 0.  A rune with nume n is (globally) enabled in the
+; current world iff either n is greater than the index-of-last-enabling or
+; array[n] is non-nil.  This is just the computation done by enabled-numep,
+; below.
 
-; The in-theory event loads the 'global-enabled-structure with
-; the theory-value and sets the index-of-last-enabling to the maximum
-; nume at that time.  This structure is passed into prove and
-; thus into rewrite, etc.
+; The in-theory event loads the 'global-enabled-structure with the theory-value
+; and sets the index-of-last-enabling to the maximum nume at that time.  This
+; structure is passed into prove and thus into rewrite, etc.
 
 ; When an in-theory hint setting is provided we change the array name
-; from ENABLED-ARRAY-j to ENABLED-ARRAY-j+1 (changing suffix
-; appropriately) and load the local theory into that structure.  After
-; we have done a few proofs with local in-theory hint settings, these
-; auxiliary arrays will have been allocated and won't be deallocated.
+; appropriately and load the local theory into that structure.  We flush each
+; such array in order to allow it to be garbage collected; see
+; restore-hint-settings-in-pspv.
 
 ; Historical Note about Nqthm
 
-; In nqthm we solved this problem by having a list of temporarily
-; disabled names which was bound when there were local enabling hint
-; settings.  That implementation suffered because if hundreds of names
-; were enabled locally the time spent searching the list was
-; excessive.  In xnqthm we solved that problem by storing the enabled
-; status on the property list of each name.  We could do that here.
-; However, that implementation suffered from the fact that if a proof
-; attempt was aborted then we had to carefully clean up the property
-; list structures so that they once again reflected the current
-; (global) theory.  The beauty of the ACL2 approach is that local hint
-; settings have no affect on the global theory and yet involve no
-; overhead.
+; In nqthm we solved this problem by having a list of temporarily disabled
+; names which was bound when there were local enabling hint settings.  That
+; implementation suffered because if hundreds of names were enabled locally the
+; time spent searching the list was excessive.  In xnqthm we solved that
+; problem by storing the enabled status on the property list of each name.  We
+; could do that here.  However, that implementation suffered from the fact that
+; if a proof attempt was aborted then we had to carefully clean up the property
+; list structures so that they once again reflected the current (global)
+; theory.  The beauty of the ACL2 approach is that local hint settings have no
+; affect on the global theory and yet involve no overhead.
 
-; A delicacy of the current implementation however concerns the
-; relation between the global enabled structure and undoing.  If the
-; world is backed up to some previous point, the
-; 'global-enabled-structure extant there is exposed and we are
-; apparently ready to roll.  However, the von Neumann array named by
-; that structure may be out-dated in the sense that it contains a now
-; undone theory.  Technically there is nothing wrong with this, but if
-; we let it persist things would be very slow because the attempt to
-; access the applicative array would detect that the von Neumann array
-; is out of date and would result in a linear search of the
-; applicative array.  We must therefore compress the applicative array
-; (and hence reload the von Neumann one) whenever we back up.
+; A delicacy of the current implementation however concerns the relation
+; between the global enabled structure and undoing.  If the world is backed up
+; to some previous point, the 'global-enabled-structure extant there is exposed
+; and we are apparently ready to roll.  However, the von Neumann array named by
+; that structure may be out-dated in the sense that it contains a now undone
+; theory.  Technically there is nothing wrong with this, but if we let it
+; persist things would be very slow because the attempt to access the
+; applicative array would detect that the von Neumann array is out of date and
+; would result in a linear search of the applicative array.  We must therefore
+; compress the applicative array (and hence reload the von Neumann one)
+; whenever we back up.
 
-; Finally, there is one last problem.  Eventually the array-size of
-; the array in one of these structures will be too small.  This
-; manifests itself when the maximum rule index at the time we load the
-; structure is equal to or greater than the array-length.  At that
-; time we grow the array size by 500.
+; Finally, there is one last problem.  Eventually the array-size of the array
+; in one of these structures will be too small.  This manifests itself when the
+; maximum rule index at the time we load the structure is equal to or greater
+; than the array-length.  At that time we grow the array size by 500.
 
-; Here is how we use an enabled structure, ens, to determine if a nume,
-; rune, or function is enabled.
+; Here is how we use an enabled structure, ens, to determine if a nume, rune,
+; or function is enabled.
 
 (defun enabled-numep (nume ens)
 
@@ -1270,12 +1261,11 @@
 
 (defun enabled-arith-numep (nume ens)
 
-; This function takes a nume (or nil) and determines if it is enabled
-; in the enabled structure ens.  We treat nil as though it were
-; enabled.  In current usage, ens is always the global arithmetic
-; theory.  Any nume created since the most recent in-arithmetic-theory
-; is considered disabled.  The normal enabled-numep would treat these
-; more recent numes as enabled.
+; This function takes a nume (or nil) and determines if it is enabled in the
+; enabled structure ens.  We treat nil as though it were enabled.  In current
+; usage, ens is always the global arithmetic theory.  Any nume created since
+; the most recent in-arithmetic-theory is considered disabled.  The normal
+; enabled-numep would treat these more recent numes as enabled.
 
 ; Our calls of the-fixnum assume that nume is less than about 2 billion.  That
 ; seems like a safe assumption!
@@ -1687,23 +1677,124 @@
                          ctx
                          state))
 
+; CLAUSE IDENTIFICATION
+
+; Before we can write the function that prints a description of
+; simplify-clause's output, we must be able to identify clauses.  This raises
+; some issues that are more understandable later, namely, the notion of the
+; pool.  See Section PUSH-CLAUSE and The Pool.
+
+; Associated with every clause in the waterfall is a unique object
+; called the clause identifier or clause-id.  These are printed out
+; at the user in a certain form, e.g.,
+
+; [3]Subgoal *2.1/5.7.9.11'''
+
+; but the internal form of these ids is:
+
+(defrec clause-id ((forcing-round . pool-lst) case-lst . primes) t)
+
+; where forcing-round is a natural number, pool-lst and case-lst are generally
+; true-lists of non-zero naturals (though elements of case-lst can be of the
+; form Dk in the case of a dijunctive split) and primes is a natural.  The
+; pool-lst is indeed a pool-lst.  (See the function pool-lst.) The case-lst is
+; structurally analogous.
+
+; A useful constant, the first clause-id:
+
+(defconst *initial-clause-id*
+
+; Note: If this changes, inspect every use of it.  As of this writing there is
+; one place where we avoid a make clause-id and use *initial-clause-id* instead
+; because we know the forcing-round is 0 and pool-lst and case-lst fields are
+; both nil and the primes field is 0.
+
+  (make clause-id
+        :forcing-round 0
+        :pool-lst nil
+        :case-lst nil
+        :primes 0))
+
+; Because of the way :DO-NOT-INDUCT name hints are implemented, and because of
+; the way we create names of theory arrays, we need to be able to produce a
+; string representing a given clause-id.  In the case of the above
+; :DO-NOT-INDUCT, we use this to form a literal atom of the form |name
+; clause-id| where clause-id is what tilde-@-clause-id-phrase will print on id.
+; Therefore, we now virtually repeat the definition of
+; tilde-@-clause-id-phrase, except this time building a string.  We could use
+; this to print all clause ids.  But that is slow because it involves consing
+; up strings.  So we suffer the inconvenience of duplication.  If
+; tilde-@-clause-id-phrase is changed, be sure to change the functions below.
+
+(defun chars-for-tilde-@-clause-id-phrase/periods (lst)
+  (declare (xargs :guard (true-listp lst)))
+  (cond
+   ((null lst) nil)
+   ((null (cdr lst)) (explode-atom (car lst) 10))
+   (t (append (explode-atom (car lst) 10)
+              (cons #\.
+                    (chars-for-tilde-@-clause-id-phrase/periods
+                     (cdr lst)))))))
+
+(defun chars-for-tilde-@-clause-id-phrase/primes (n)
+  (declare (xargs :guard (and (integerp n) (>= n 0))))
+  (cond ((= n 0) nil)
+        ((= n 1) '(#\'))
+        ((= n 2) '(#\' #\'))
+        ((= n 3) '(#\' #\' #\'))
+        (t (cons #\' (append (explode-atom n 10) '(#\'))))))
+
+(defun chars-for-tilde-@-clause-id-phrase (id)
+  (append
+   (if (= (access clause-id id :forcing-round) 0)
+       nil
+     `(#\[ ,@(explode-atom (access clause-id id :forcing-round) 10) #\]))
+   (cond ((null (access clause-id id :pool-lst))
+          (cond ((null (access clause-id id :case-lst))
+                 (append '(#\G #\o #\a #\l)
+                         (chars-for-tilde-@-clause-id-phrase/primes
+                          (access clause-id id :primes))))
+                (t (append '(#\S #\u #\b #\g #\o #\a #\l #\Space)
+                           (chars-for-tilde-@-clause-id-phrase/periods
+                            (access clause-id id :case-lst))
+                           (chars-for-tilde-@-clause-id-phrase/primes
+                            (access clause-id id :primes))))))
+         (t (append
+             '(#\S #\u #\b #\g #\o #\a #\l #\Space #\*)
+             (chars-for-tilde-@-clause-id-phrase/periods
+              (access clause-id id :pool-lst))
+             (cons #\/
+                   (append (chars-for-tilde-@-clause-id-phrase/periods
+                            (access clause-id id :case-lst))
+                           (chars-for-tilde-@-clause-id-phrase/primes
+                            (access clause-id id :primes)))))))))
+
+(defun string-for-tilde-@-clause-id-phrase (id)
+
+; Warning: Keep this in sync with tilde-@-clause-id-phrase.
+
+  (coerce (chars-for-tilde-@-clause-id-phrase id)
+          'string))
+
 (defun load-theory-into-enabled-structure
-  (theory-expr theory augmented-p ens incrmt-array-name-flg
+  (theory-expr theory augmented-p ens incrmt-array-name-info
                index-of-last-enabling wrld ctx state)
 
 ; Note: Theory must be a runic theory if augmented-p is nil and otherwise an
 ; augmented runic theory, but never a common theory.
 
 ; We do exactly what the name of this function says, we load the given theory
-; into the enabled structure ens.  If incrmt-array-name-flg is t we increment
-; the array name suffix.  Otherwise, we use the same name.  Loading consists of
-; augmenting the theory (if augmented-p is nil) to convert it into a list of
-; pairs, (nume . rune), mapping numes to their runes, and then compressing it
-; into the named array.  We set the index of last enabling to be the highest
-; existing nume in wrld right now unless index-of-last-enabling is non-nil, in
-; which case we use that (which should be a natp).  Thus, any name introduced
-; after this is enabled relative to this ens.  If the array of the ens is too
-; short, we extend it by 500.
+; into the enabled structure ens.  If incrmt-array-name-info is t we increment
+; the array name suffix.  If incrmt-array-name-info is non-boolean, then it is
+; a clause-id that we use to create a new name uniquely determined by that
+; clause-id.  Otherwise, we use the same name.  Loading consists of augmenting
+; the theory (if augmented-p is nil) to convert it into a list of pairs, (nume
+; . rune), mapping numes to their runes, and then compressing it into the named
+; array.  We set the index of last enabling to be the highest existing nume in
+; wrld right now unless index-of-last-enabling is non-nil, in which case we use
+; that (which should be a natp).  Thus, any name introduced after this is
+; enabled relative to this ens.  If the array of the ens is too short, we
+; extend it by 500.
 
 ; A Refresher Course on ACL2 One Dimensional Arrays:
 
@@ -1724,15 +1815,22 @@
          (new-d (cond ((< n d) d)
                       (t (+ d (* 500 (1+ (floor (- n d) 500)))))))
          (root (access enabled-structure ens :array-name-root))
-         (suffix (cond (incrmt-array-name-flg
+         (suffix (cond ((eq incrmt-array-name-info t)
                         (1+ (access enabled-structure ens :array-name-suffix)))
                        (t (access enabled-structure ens :array-name-suffix))))
-         (name (cond (incrmt-array-name-flg
+         (name (cond ((eq incrmt-array-name-info t)
                       (intern (coerce
                                (append root
                                        (explode-nonnegative-integer suffix
                                                                     10
                                                                     nil))
+                               'string)
+                              "ACL2"))
+                     (incrmt-array-name-info ; must be a clause-id
+                      (intern (coerce
+                               (append root
+                                       (chars-for-tilde-@-clause-id-phrase
+                                        incrmt-array-name-info))
                                'string)
                               "ACL2"))
                      (t (access enabled-structure ens :array-name))))
@@ -5424,43 +5522,35 @@
           (term-and-typ-to-lookup hyp wrld)
           (search-type-alist term typ type-alist unify-subst ttree wrld)))
 
-(mutual-recursion
+(defun bind-free-vars-to-unbound-free-vars (vars alist)
 
-(defun sublis-var-and-mark-free (alist form)
+; For every var in vars that is not bound in alist, create the binding
+; (var . UNBOUND-FREE-var) and add that binding to alist.  Return the
+; extended alist.  We use this function to instantiate free vars in
+; FORCEd and CASE-SPLIT hypotheses.  In that application, vars will be
+; the list of all vars occuring in the hyp and alist will be the
+; unify-subst.  The name ``unbound free var'' is a little odd out of
+; context but we hope it will make the user realize that the variable
+; occurred freely and we couldn't find a binding for it to make the hyp
+; true before forcing or splitting.
 
-; This function is rather odd: it is equivalent to (sublis-var alist'
-; form) where alist' is derived from alist by adding a pair (var .
-; ???-var) for each variable var in form that is not assigned a value
-; by alist.  Thus it creates an instance of form.  However, the free
-; vars of form are assigned essentially arbitrary variable values and
-; while no two free vars are identified by this process, there is no
-; guarantee that the variables introduced in their stead are "new."
-; For example, ???-var may come into the instantiated term via alist.
-; The only reason for this function is to highlight the free vars in a
-; term upon which we will split, in the half-hearted hope that the
-; user will spot it.
-
-  (cond ((variablep form)
-         (let ((a (assoc-eq form alist)))
-           (cond (a (cdr a))
-                 (t (packn (list "???-" form))))))
-        ((fquotep form)
-         form)
-        (t (cons-term (ffn-symb form)
-                      (sublis-var-and-mark-free-lst alist (fargs form))))))
-
-(defun sublis-var-and-mark-free-lst (alist l)
-  (if (null l)
-      nil
-    (cons (sublis-var-and-mark-free alist (car l))
-          (sublis-var-and-mark-free-lst alist (cdr l)))))
-
-)
+  (cond ((endp vars) alist)
+        ((assoc-eq (car vars) alist)
+         (bind-free-vars-to-unbound-free-vars (cdr vars) alist))
+        (t (bind-free-vars-to-unbound-free-vars
+            (cdr vars)
+            (cons (cons (car vars)
+                        (packn (list "UNBOUND-FREE-" (car vars))))
+                  alist)))))
 
 ; The Accumulated Persistence Essay
 
-; We now develop the code needed to track accumulated-persistence.
-; To activate accumulated-persistence, you must first call
+; We now develop the code needed to track accumulated-persistence.  The
+; documentation topic for accumulated-persistence serves as a useful
+; introduction to what is implemented by the code, and is a good starting point
+; before reading this Essay.
+
+; A typical use of this utility is as follows.
 
 ; >(accumulated-persistence t)              ; activate and initialize
 ; > ...                                     ; do proofs
@@ -5483,6 +5573,9 @@
 ; where k is 1, we naturally use a let instead of an mv-let.)  However, we
 ; insert some additional code to accumulate the persistence of rune.
 
+; There are optional arguments of with-accumulated-persistence not described in
+; this essay, but whose meaning is pretty clear from the code.
+
 ; The implementation of accumulated-persistence is as follows.  First, the
 ; necessary global data structures are maintained as the status of a wormhole
 ; called 'accumulated-persistence.  As usual with a wormhole status, it is of
@@ -5498,6 +5591,73 @@
 ; kept in a single accp-info record, which is the value of the wormhole-data
 ; field of wormhole-status:
 
+; If accumulated persistence is enabled then we give special treatment to
+; hypotheses and conclusions of rules.  Each is represented as an ``extended
+; rune'' (``xrune''), which provides an accumulation site for work done on
+; behalf of that hypothesis or conclusion.  Thus, we actually traffic in
+; xrunes, where an xrune is either a rune, a hyp-xrune (:hyp rune , n) where n
+; is a positive integer, or a conc-xrune (:conc . rune).  The hyp-xrune (:hyp
+; rune . n) is used in accumulated-persistence for recording the work done on
+; behalf of the nth hypothesis of rune, while the conc-xrune (:conc . rune)
+; records the work done on behalf of the right-hand-side of the rune.  Note
+; that :doc accumulated-persistence says that a hyp-xrune is (:hyp n . rune)
+; rather than (:hyp rune . n), but we found the latter form much more
+; convenient for sorting.  Still, we present (:hyp n . rune) to the user by
+; calling prettyify-xrune.
+
+(defabbrev x-xrunep (xrune) ; extended xrunep
+  (or (eq (car xrune) :hyp)
+      (eq (car xrune) :conc)))
+
+(defabbrev hyp-xrune (n rune)
+  (assert$ (not (x-xrunep rune))
+           (list* :hyp rune n)))
+
+(defabbrev hyp-xrune-rune (xrune)
+  (assert$ (and (x-xrunep xrune)
+                (eq (car xrune) :hyp))
+           (cadr xrune)))
+
+(defabbrev conc-xrune (rune)
+  (assert$ (not (x-xrunep rune))
+           (list* :conc rune)))
+
+(defabbrev conc-xrune-rune (xrune)
+  (assert$ (and (x-xrunep xrune)
+                (eq (car xrune) :conc))
+           (cdr xrune)))
+
+(defabbrev xrune-rune (xrune)
+  (cond ((x-xrunep xrune)
+         (if (eq (car xrune) :hyp)
+             (cadr xrune)
+           (cdr xrune)))
+        (t xrune)))
+
+(defabbrev rune= (rune1 rune2)
+  (and (eq (car rune1) (car rune2))
+       (equal (cdr rune1) (cdr rune2))))
+
+(defabbrev xrune= (xrune1 xrune2)
+  (cond ((eq (car xrune1) :hyp)
+         (and (eq (car xrune2) :hyp)
+              (rune= (cadr xrune1) (cadr xrune2))
+              (eql (cddr xrune1) (cddr xrune2))))
+        ((eq (car xrune1) :conc)
+         (and (eq (car xrune2) :conc)
+              (rune= (cdr xrune1) (cdr xrune2))))
+        (t (rune= xrune1 xrune2))))
+
+(defun prettyify-xrune (xrune)
+
+; We sort :hyp xrunes first by their rune (see sort-xrune-alist-by-rune), which
+; is why a hyp xrune is of the form (:hyp rune . n) rather than (:hyp n
+; . rune).  But the latter is more pleasant to view.
+
+  (cond ((eq (car xrune) :hyp)
+         (list* :hyp (cddr xrune) (cadr xrune)))
+        (t xrune)))
+
 (defrec accp-info
 
 ; The "s" and "f" suffixes below suggest "success" and "failure", though a
@@ -5506,7 +5666,8 @@
 ; description of fields.
 
   (((cnt-s . cnt-f) . (stack-s . stack-f))
-   rune-stack
+   xrune-stack
+   xrunep
    .
    totals)
   t)
@@ -5519,51 +5680,90 @@
 
 ; Stack-s (resp. stack-f) is a stack of old values of cnt-s (resp. cnt-f).
 
-; Rune-stack is a list of runes corresponding to stack-s and stack-f, where
-; each rune corresponds to a call of push-accp made on behalf of that rune.
+; Xrune-stack is a list of xrunes corresponding to stack-s and stack-f, where
+; each xrune corresponds to a call of push-accp made on behalf of that xrune.
+
+; Xrunep is true if we are to collect information for hypothesis and conclusion
+; xrunes, and is nil otherwise.
 
 ; Totals is a stack of the accumulated totals, initially '(nil); it is one
 ; longer than the common length of stack-s and stack-f.  Each element of the
-; stack is a list associating runes with totals accumulated for a corresponding
-; rune (i.e., an ancestral call of push-accp), as follows.
+; stack is a list associating xrunes with totals accumulated for a
+; corresponding xrune (i.e., an ancestral call of push-accp), as follows.
 
 (defrec accp-entry
+
+; Warning.  We construct lists of such entries that we refer to as alists.
+; Before changing the shape of this record, consider whether we are relying on
+; it being a record whose car is its :xrune field.  See for example
+; sort-xrune-alist-by-rune1.
 
 ; The "s" and "f" suffixes below suggest "success" and "failure", though a
 ; better distinction is between "useful work" and "useless work".  Our
 ; user-level reports say "useful" and "useless".  See just below for a further
 ; description of the fields.
 
-  (rune . ((n-s . ap-s)
-           .
-           (n-f . ap-f)))
+  (xrune . ((n-s . ap-s)
+            .
+            (n-f . ap-f)))
   t)
 
 ; Each element of stack-s (resp. stack-f) corresponds to an attempt to apply a
-; certain rune and the element is the value of cnt-s (resp. cnt-f) at the time
+; certain xrune and the element is the value of cnt-s (resp. cnt-f) at the time
 ; the attempt started.  When the attempt is successful, we increase cnt-s,
-; first by one and then by the difference of the current value of cnt-s with
-; the old value (on top of stack-s) to find out how many lemmas were usefully
-; tried under that rune, and we accumulate that difference into the success
-; fields of the current totals for that rune; similarly for cnt-f and useless
-; tries.  When the attempt fails, all accumulation is into the failure
-; (useless) fields of the totals.  The accumulated totals is a stack of lists,
-; each of which contains elements associating runes with values n-s, ap-s, n-f,
-; and ap-f, where n-s is the number of times rune was pushed onto the stack and
-; successfully applied, ap-s is the accumulated persistence of useful
-; applications of that rune (the total number of applications while that rune
-; was on the stack, not yet including such applications that are recorded in
-; more recent stack frames), and n-f and ap-f are similar but for failed
-; applications of that rune.
+; first by one if we have a rune rather than a hyp-xrune or conc-xrune, and then
+; by the difference of the current value of cnt-s with the old value (on top of
+; stack-s) to find out how many lemmas were usefully tried under that xrune,
+; and we accumulate that difference into the success fields of the current
+; totals for that xrune; similarly for cnt-f and useless tries.  When the
+; attempt fails, all accumulation is into the failure (useless) fields of the
+; totals.  The accumulated totals is a stack of lists, each of which contains
+; elements associating xrunes with values n-s, ap-s, n-f, and ap-f, where n-s
+; is the number of times xrune was pushed onto the stack and successfully
+; applied, ap-s is the accumulated persistence of useful applications of that
+; xrune (the total number of applications while that xrune was on the stack,
+; not yet including such applications that are recorded in more recent stack
+; frames), and n-f and ap-f are similar but for failed applications of that
+; xrune.
 
 ; Performance: We have seen (Version_3.2.1) about a 50% increase in time with
-; accumulated-persistence turned on, in very limited experiments.
+; accumulated-persistence turned on, in very limited experiments.  In later
+; versions we have found a significantly smaller increase unless enhanced
+; statistics are gathered.  Here are results using code developed after
+; Version_4.1, using Allegro CL.
 
-(defabbrev rune= (rune1 rune2)
-  (and (eq (car rune1) (car rune2))
-       (equal (cdr rune1) (cdr rune2))))
+#||
+In directory /projects/acl2/devel/books/workshops/2004/legato/support/
+(see below for discussion of which forms were submitted for each experiment).
 
-(defun merge-accumulated-persistence-aux (rune entry alist)
+(set-inhibit-output-lst '(prove proof-tree))
+;; (ld "/projects/acl2/devel-misc/patches/accumulated-persistence-hyps-rhs/patch.lisp")
+;; (value :q)
+;;; (load "/projects/acl2/devel-misc/patches/accumulated-persistence-hyps-rhs/patch.fasl")
+;; (load "/projects/acl2/devel-misc/patches/accumulated-persistence-hyps-rhs/old.fasl")
+;; (lp)
+; (accumulated-persistence t)
+(time$ (ld "proof-by-generalization-mult.lisp"))
+
+No accp (skip commented forms)
+; 97.01 seconds realtime, 95.54 seconds runtime.
+
+Old accp (include only one commented form, (accumulated-persistence t))
+; 114.82 seconds realtime, 113.46 seconds runtime.
+
+New accp (include all commented forms except ;;;)
+; 164.95 seconds realtime, 163.69 seconds runtime.
+
+New accp (include all commented forms)
+; 165.09 seconds realtime, 163.90 seconds runtime.
+
+The results above were based on code that always gave results for a :conc
+xrune.  We now skip that xrune if there are no hypotheses, but that didn't make
+much difference:
+; 164.84 seconds realtime, 163.50 seconds runtime.
+||#
+
+(defun merge-accumulated-persistence-aux (xrune entry alist)
   (cond ((endp alist)
 
 ; See the comment below merge-accumulated-persistence for an attempt we made to
@@ -5571,9 +5771,9 @@
 ; rather than just pushing the entry on the front).
 
          (list entry))
-        ((rune= rune (access accp-entry (car alist) :rune))
+        ((xrune= xrune (access accp-entry (car alist) :xrune))
          (cons (make accp-entry
-                     :rune rune
+                     :xrune xrune
                      :n-s (+ (access accp-entry entry :n-s)
                              (access accp-entry (car alist) :n-s))
                      :ap-s (+ (access accp-entry entry :ap-s)
@@ -5584,21 +5784,21 @@
                               (access accp-entry (car alist) :ap-f)))
                (cdr alist)))
         (t (cons (car alist)
-                 (merge-accumulated-persistence-aux rune entry (cdr alist))))))
+                 (merge-accumulated-persistence-aux xrune entry (cdr alist))))))
 
 (defun merge-accumulated-persistence-rec (new-alist old-alist)
   (cond ((endp new-alist) old-alist)
         (t (merge-accumulated-persistence-rec
             (cdr new-alist)
             (merge-accumulated-persistence-aux
-             (access accp-entry (car new-alist) :rune)
+             (access accp-entry (car new-alist) :xrune)
              (car new-alist)
              old-alist)))))
 
 (defun merge-accumulated-persistence (new-alist old-alist)
 
-; We tried an approach using sorting with rune-<, but it was much more
-; expensive.  We used as an example:
+; We tried an approach using sorting with rune-< (before we considered xrunes),
+; but it was much more expensive.  We used as an example:
 ; cd books/workshops/2004/legato/support/
 ; acl2::(set-inhibit-output-lst '(prove proof-tree))
 ; (accumulated-persistence t)
@@ -5633,6 +5833,9 @@
         (t (merge-accumulated-persistence-rec new-alist old-alist))))
 
 #||
+
+This multi-line comment was written before the introduction of xrunes, and we
+have left it unchanged from that time.
 
 The following alternate code doesn't do as well, even though it uses nconc.
 The nconc version doesn't even seem much better on space (in fact worse in an
@@ -5705,20 +5908,20 @@ gbc time        :      8.930 secs
 
 ||#
 
-(defun add-accumulated-persistence-s (rune delta-s delta-f alist original-alist
-                                           acc)
+(defun add-accumulated-persistence-s (xrune delta-s delta-f alist
+                                            original-alist acc)
 
 ; Warning: Keep this in sync with add-accumulated-persistence-f.
 
   (cond ((null alist)
          (cons (make accp-entry
-                     :rune rune
+                     :xrune xrune
                      :n-s  1
                      :ap-s (+ delta-f delta-s)
                      :n-f  0
                      :ap-f 0)
                original-alist))
-        ((rune= rune (access accp-entry (car alist) :rune))
+        ((xrune= xrune (access accp-entry (car alist) :xrune))
          (cons (change accp-entry (car alist)
                        :ap-f 0 ; no change in :n-f
                        :n-s  (1+ (access accp-entry (car alist) :n-s))
@@ -5729,11 +5932,11 @@ gbc time        :      8.930 secs
                                         :ap-f)))
                (revappend acc (cdr alist))))
         (t (add-accumulated-persistence-s
-            rune delta-s delta-f (cdr alist) original-alist
+            xrune delta-s delta-f (cdr alist) original-alist
             (cons (car alist) acc)))))
 
-(defun add-accumulated-persistence-f (rune delta-s delta-f alist original-alist
-                                           acc)
+(defun add-accumulated-persistence-f (xrune delta-s delta-f alist
+                                            original-alist acc)
 
 ; Warning: Keep this in sync with add-accumulated-persistence-s.
 
@@ -5742,13 +5945,13 @@ gbc time        :      8.930 secs
 
   (cond ((null alist)
          (cons (make accp-entry
-                     :rune rune
+                     :xrune xrune
                      :n-s  0
                      :ap-s 0
                      :n-f  1
                      :ap-f (+ delta-f delta-s))
                original-alist))
-        ((rune= rune (access accp-entry (car alist) :rune))
+        ((xrune= xrune (access accp-entry (car alist) :xrune))
          (cons (change accp-entry (car alist)
                        :n-f  (1+ (access accp-entry (car alist) :n-f))
                        :ap-f (assert$
@@ -5759,7 +5962,7 @@ gbc time        :      8.930 secs
                                          :ap-f))))
                (revappend acc (cdr alist))))
         (t (add-accumulated-persistence-f
-            rune delta-s delta-f (cdr alist) original-alist
+            xrune delta-s delta-f (cdr alist) original-alist
             (cons (car alist) acc)))))
 
 (defun accumulated-persistence-make-failures (alist)
@@ -5774,13 +5977,14 @@ gbc time        :      8.930 secs
                        :ap-s 0)
                (accumulated-persistence-make-failures (cdr alist))))))
 
-(defun add-accumulated-persistence (rune success-p delta-s delta-f alist-stack)
+(defun add-accumulated-persistence (xrune success-p delta-s delta-f
+                                          alist-stack)
 
 ; Alist-stack is a list of lists of accp-entry records.  First, we modify the
 ; top of alist-stack to record everything as useless (failure) if success-p is
 ; nil.  Then, we merge that modification into the second element of
-; alist-stack, after incrementing by 1 for the given rune's :n-s or :n-f and by
-; delta for its :ap-s or :ap-f, according to success-p.
+; alist-stack, after incrementing by 1 for the given xrune's :n-s or :n-f and
+; by delta for its :ap-s or :ap-f, according to success-p.
 
   (assert$
    (cdr alist-stack)
@@ -5790,10 +5994,10 @@ gbc time        :      8.930 secs
           (new-alist (cond
                       (success-p
                        (add-accumulated-persistence-s
-                        rune delta-s delta-f alist alist nil))
+                        xrune delta-s delta-f alist alist nil))
                       (t
                        (add-accumulated-persistence-f
-                        rune delta-s delta-f alist alist nil)))))
+                        xrune delta-s delta-f alist alist nil)))))
      (cons (merge-accumulated-persistence new-alist (cadr alist-stack))
            (cddr alist-stack)))))
 
@@ -5823,8 +6027,11 @@ gbc time        :      8.930 secs
                                            ; below).  The `a' versions avoid
                                            ; showing the useful/useless
                                            ; breakdown.
-  
+
   ~ev[]~/
+
+  See the end of this item for a discussion of ``enhanced statistics
+  gathering,'' which can be useful for more fine-grained proof debugging.
 
   Generally speaking, the more ACL2 knows, the slower it runs.  That is because
   the search space grows with the number of alternative rules.  Often, the
@@ -5854,22 +6061,22 @@ gbc time        :      8.930 secs
 
   Consider a ~c[:]~ilc[rewrite] rule named ~ilc[rune].  For simplicity, let us
   imagine that ~ilc[rune] is tried only once in the period during which
-  accumulated persistence is being ~il[monitor]ed.  Recall that to apply a
-  rewrite rule we must match the left-hand side of the conclusion to some term
-  we are trying to rewrite, establish the hypotheses of ~ilc[rune] by
-  rewriting, and, if successful, then rewrite the right-hand side of the
-  conclusion.  We say ~ilc[rune] is ``being tried'' from the time we have
-  matched its left-hand side to the time we have either abandoned the attempt
-  or finished rewriting its right-hand side.  (By ``match'' we mean to include
-  any loop-stopper requirement; ~pl[loop-stopper].)  During that period of time
-  other rules might be tried, e.g., to establish the hypotheses.  The rules
-  tried while ~ilc[rune] is being tried are ``billed'' to ~ilc[rune] in the
-  sense that they are being considered here only because of the demands of
-  ~ilc[rune].  Thus, if no other rules are tried during that period, the
-  accumulated persistence of ~ilc[rune] is ~c[1] ~-[] we ``bill'' ~ilc[rune]
-  once for its own application attempt.  If, on the other hand, we tried ~c[10]
-  rules on behalf of that application of ~ilc[rune], then ~ilc[rune]'s
-  accumulated persistence would be ~c[11].
+  accumulated persistence is being monitored.  Recall that to apply a rewrite
+  rule we must match the left-hand side of the conclusion to some term we are
+  trying to rewrite, establish the hypotheses of ~ilc[rune] by rewriting, and,
+  if successful, then rewrite the right-hand side of the conclusion.  We say
+  ~ilc[rune] is ``being tried'' from the time we have matched its left-hand
+  side to the time we have either abandoned the attempt or finished rewriting
+  its right-hand side.  (By ``match'' we mean to include any loop-stopper
+  requirement; ~pl[loop-stopper].)  During that period of time other rules
+  might be tried, e.g., to establish the hypotheses.  The rules tried while
+  ~ilc[rune] is being tried are ``billed'' to ~ilc[rune] in the sense that they
+  are being considered here only because of the demands of ~ilc[rune].  Thus,
+  if no other rules are tried during that period, the accumulated persistence
+  of ~ilc[rune] is ~c[1] ~-[] we ``bill'' ~ilc[rune] once for its own
+  application attempt.  If, on the other hand, we tried ~c[10] rules on behalf
+  of that application of ~ilc[rune], then ~ilc[rune]'s accumulated persistence
+  would be ~c[11].
 
   One way to envision accumulated persistence is to imagine that every
   time a ~il[rune] is tried it is pushed onto a stack.  The rules tried on
@@ -6009,6 +6216,151 @@ gbc time        :      8.930 secs
   There are other subtleties in how rune applications are tallied, documented
   elsewhere:  ~pl[accumulated-persistence-subtleties].
 
+  We conclude with a discussion of ``enhanced'' statistics gathering, which is
+  enabled by supplying ~c[accumulated-persistence] the argument ~c[:ALL]:
+  ~bv[]
+  (accumulated-persistence :all)
+  ~ev[]
+  At some additional performance expense (but probably well under a factor of
+  2 altogether), ACL2 then gathers additional statistics for individual
+  hypotheses of rules as well as their conclusions.  To understand how this
+  works, suppose ~c[rn] is a ~il[rune].  Then we prepend the keyword ~c[:CONC]
+  to ~c[rn] to form what we call its ``conclusion xrune'', and for its ~c[I]-th
+  hypothesis we prepend ~c[:HYP I] to ~c[rn] to form its ~c[I]-th ``hypothesis
+  xrune.''  Here, ``xrune'' is pronounced ``ex rune'', and is mnemonic for
+  ``extended rune.''  For example, if ~c[(REWRiTE FOO)] is a ~il[rune] then
+  ~c[(:CONC REWRiTE FOO)] is its conclusion xrune, and ~c[(:HYP 2 REWRiTE FOO)]
+  is a hypothesis xrune corresponding to the second hypothesis of the
+  corresponding rewrite rule.
+
+  With ~c[(accumulated-persistence :all)], we instruct ACL2 to track not only
+  runes but also xrunes.  Then, ~c[(show-accumulated-persistence)] will display
+  information for all xrunes in a format that we consider to be ``raw'', in the
+  sense that data for xrunes are displayed just as for runes.  But a ``merged''
+  format is also available.  Here is a summary of display commands, followed
+  below by further discussion.
+
+  ~bv[]
+    (show-accumulated-persistence :frames t) ; t is optional, i.e., the default
+       ; Display enhanced statistics sorted by frames, in a ``raw'' format.
+    (show-accumulated-persistence :frames :merge)
+       ; Display enhanced statistics sorted by frames, in a ``merged'' format.
+    (show-accumulated-persistence :frames nil)
+       ; Display regular statistics sorted by frames, without the enhancements.
+
+    ; More generally, the descriptions just above apply for any legal first
+    ; argument:
+
+    (show-accumulated-persistence KEY t)
+    (show-accumulated-persistence KEY :merge)
+    (show-accumulated-persistence KEY nil)
+
+    ; Note also these alternate forms, equivalent to the first of the two forms
+    ; just above, i.e., the form with second argument of t:
+    (show-accumulated-persistence KEY :raw)
+    (show-accumulated-persistence KEY)
+  ~ev[]
+
+  There is a significant difference between how runes are tracked and how ACL2
+  tracks hypothesis and conclusion xrunes: unlike regular runes, these xrunes
+  do not contribute to the accumulated ~c[:frames] counts.  Rather, they serve
+  as accumulation sites without contributing their ~c[:tries] to any
+  accumulation.  Consider for example the snippet below, taken from a report
+  created with the ~c[:merge] option (to be discussed further below), i.e., by
+  evaluating the form ~c[(show-accumulated-persistence :frames :merge)].
+  ~bv[]
+     :frames   :tries    :ratio  rune
+     --------------------------------
+         462      211 (    2.18) (:REWRITE PERM-MEM)
+          13        6    [useful]
+         449      205    [useless]
+        .............................
+         251       47 (    5.34) (:HYP 2 :REWRITE PERM-MEM)
+           6        6    [useful]
+         245       41    [useless]
+        .............................
+           0      211 (    0.00) (:HYP 1 :REWRITE PERM-MEM)
+           0        6    [useful]
+           0      205    [useless]
+        .............................
+           0        7 (    0.00) (:CONC :REWRITE PERM-MEM)
+           0        6    [useful]
+           0        1    [useless]
+     --------------------------------
+  ~ev[]
+  Notice that while ~c[:tries] are recorded for the xrune
+  ~c[(:HYP 1 :REWRITE PERM-MEM)], no ~c[:frames] are recorded.  This is because
+  no stack frames were built for runes while this xrune was on the stack ~-[]
+  only for the xrune itself, which as we explained above is not accumulated
+  into the total ~c[:frames] counts.  As it turns out, this lack of stack
+  frames is explained by the fact that the rewrite rule ~c[PERM-MEM] has a free
+  variable in the first hypothesis.
+  ~bv[]
+  ACL2 !>:pe perm-mem
+           18  (DEFTHM PERM-MEM
+                       (IMPLIES (AND (PERM X Y) (MEM A X))
+                                (MEM A Y))
+                       :RULE-CLASSES ((:REWRITE :MATCH-FREE :ONCE)))
+  ACL2 !>
+  ~ev[]
+  The second hypothesis, however, does cause additional rewriting in order to
+  rewrite it to true, resulting in 251 stack frames for runes.  We see that the
+  conclusion does not lead to creation any rune stack frames, which might seem
+  to suggest that only 251 stack frames for runes were created on behalf of
+  this rule application ~-[] yet, we see that 462 frames were actually
+  created.  The difference is the 211 frames created for the rewrite rule
+  itself.  Even if the total had been a bit more than 462, one need not be
+  surprised, as there could be some work recorded during application of the
+  rewrite rule, such as type-prescription reasoning, that is not done during
+  rewriting of a hypothesis or the conclusion.
+
+  Now suppose we have executed ~c[(accumulated-persistence :all)] and attempted
+  some proofs, and now we are ready to see statistics.  The form
+  ~c[(show-accumulated-persistence)] displays statistics exactly as described
+  above, treating these extra xrunes just as though they are runes; similarly
+  for the form ~c[(show-accumulated-persistence KEY)], for any legal ~c[KEY].
+  A second optional argument may however be supplied to
+  ~c[show-accumulated-persistence].  The default for that second argument is
+  ~c[t], and a second argument of ~c[:raw] is treated the same as ~c[t]; thus,
+  these arguments provide the behavior just described, where data for xrunes
+  are displayed just as for runes.  You may restrict output to runes, ignoring
+  hypothesis and conclusion xrunes, by giving a second argument of ~c[nil].
+  (This gives the same behavior as if we had started with the command
+  ~c[(accumulated-persistence t)] instead of the command
+  ~c[(accumulated-persistence :all)].)  Finally, you may give a second argument
+  of ~c[:merge], in which case output will be sorted and displayed as though
+  only runes were tracked (not the extra xrunes), but each data item for a
+  non-rune xrune will be merged so that it is displayed in suitable order just
+  below its corresponding rune, as in the ~c[PERM-MEM] example displayeda
+  above.
+
+  We close by mentioning two aspect of enhanced statistics display for
+  ~c[:CONC] xrunes that have potential to be confusing.  First consider the
+  following example.
+  ~bv[]
+       :frames   :tries    :ratio  rune
+     --------------------------------
+          14        4 (    3.50) (:REWRITE DEFAULT-+-2)
+           0        0    [useful]
+          14        4    [useless]
+        .............................
+          10        4 (    2.50) (:HYP 1 :REWRITE DEFAULT-+-2)
+           0        0    [useful]
+          10        4    [useless]
+     --------------------------------
+  ~ev[]
+  It may be surprising that no data is displayed for the corresponding
+  ~c[:CONC] xrune.  The explanation, however, is simple: the hypothesis never
+  rewrote to true, so the conclusion was never rewritten.  This is consistent
+  with the marking as ``useless'' of all ~c[:frames] and ~c[:tries] for the
+  rune and the hypothesis xrune.  Note by the way, once again, that the
+  hypothesis xrune does not contribute to any ~c[:frames] count.
+
+  Another reason not to see data displayed for a ~c[:CONC] xrune is that if a
+  rule has no hypotheses, then no such data is collected.  This decision was
+  made because in the case of no hypotheses, we expect it to be very rare that
+  information for the ~c[:CONC] xrune will add any useful insight.
+
   Users are encouraged to think about other meters we could install in ACL2 to
   help diagnose performance problems."
 
@@ -6016,18 +6368,23 @@ gbc time        :      8.930 secs
 ; accumulated-persistence wormhole is non-nil.  If accummulated persistence is
 ; not enabled, the data is nil.
 
-  `(wormhole-eval 'accumulated-persistence
-                  '(lambda (whs)
-                     (set-wormhole-data whs
-                       (if ,flg
-                            (make accp-info
-                                  :cnt-s 0
-                                  :cnt-f 0
-                                  :stack-s nil
-                                  :stack-f nil
-                                  :totals '(nil))
-                            nil)))
-                  nil))
+  (declare (xargs :guard (member-equal flg '(t 't nil 'nil :all ':all))))
+  (let* ((flg (if (consp flg) (cadr flg) flg))
+         (collect-hyp-and-conc-xrunes (eq flg :all)))
+    `(wormhole-eval
+      'accumulated-persistence
+      '(lambda (whs)
+         (set-wormhole-data whs
+                            (if ,flg
+                                (make accp-info
+                                      :cnt-s 0
+                                      :cnt-f 0
+                                      :stack-s nil
+                                      :stack-f nil
+                                      :xrunep ,collect-hyp-and-conc-xrunes
+                                      :totals '(nil))
+                              nil)))
+      nil)))
 
 (defdoc accumulated-persistence-subtleties
 
@@ -6171,11 +6528,14 @@ gbc time        :      8.930 secs
         (t (merge-car-> (merge-sort-car-> (evens l))
                         (merge-sort-car-> (odds l))))))
 
-(defconst *accp-separator*
+(defconst *accp-major-separator*
   "   --------------------------------~%")
 
+(defconst *accp-minor-separator*
+  "      .............................~%")
+
 (defun show-accumulated-persistence-phrase0 (entry key)
-  (let* ((rune (access accp-entry entry :rune))
+  (let* ((xrune (access accp-entry entry :xrune))
          (n-s (access accp-entry entry :n-s))
          (n-f (access accp-entry entry :n-f))
          (n (+ n-s n-f))
@@ -6189,7 +6549,7 @@ gbc time        :      8.930 secs
                 (cons (floor ap n) 5)
                 (mod (floor (* 10 ap) n) 10)
                 (mod (floor (* 100 ap) n) 10)
-                rune)))
+                (prettyify-xrune xrune))))
       (case key
         ((:useless :ratio-a :frames-a :tries-a)
          (list main-msg))
@@ -6200,81 +6560,238 @@ gbc time        :      8.930 secs
                     (cons n-s 8))
                (msg "~c0 ~c1    [useless]~%"
                     (cons ap-f 10)
-                    (cons n-f 8))
-               *accp-separator*))))))
+                    (cons n-f 8))))))))
 
-(defun show-accumulated-persistence-phrase1 (key alist acc)
+(defun show-accumulated-persistence-phrase1 (key alist mergep acc)
 
 ; Alist has element of the form (x . accp-entry), where x is the key upon which
-; we sorted.
+; we sorted.  Last-rune is true (initally t, generally a rune) if and only if
+; we are calling show-accumulated-persistence with display = :merge.
 
   (cond ((null alist) acc)
         (t (show-accumulated-persistence-phrase1
             key
             (cdr alist)
-            (if (and (eq key :useless)
-                     (not (eql (access accp-entry (cdr (car alist))
-                                       :ap-s)
-                               0)))
-                acc
-              (append (show-accumulated-persistence-phrase0 (cdr (car alist))
-                                                            key)
-                      acc))))))
+            mergep
+            (cons (cond ((and mergep
+                              (cdr alist)
+                              (equal (xrune-rune
+                                      (access accp-entry
+                                              (cdr (car (cdr alist)))
+                                              :xrune))
+                                     (xrune-rune
+                                      (access accp-entry
+                                              (cdr (car alist))
+                                              :xrune))))
 
-(defun show-accumulated-persistence-phrase2 (key alist)
+; The next entry to process for extending the accumulator has the same rune as
+; the current entry in this case.
+
+                         *accp-minor-separator*)
+                        (t *accp-major-separator*))
+                  (append (show-accumulated-persistence-phrase0
+                           (cdr (car alist))
+                           key)
+                          acc))))))
+
+(defun show-accumulated-persistence-remove-useless (alist acc)
+  (cond ((null alist) (reverse acc))
+        ((not (eql (access accp-entry (cdr (car alist))
+                           :n-s)
+                   0))
+         (show-accumulated-persistence-remove-useless (cdr alist) acc))
+        (t (show-accumulated-persistence-remove-useless
+            (cdr alist)
+            (cons (car alist) acc)))))
+
+(defun show-accumulated-persistence-phrase-key (key entry lastcdr)
+  (let* ((ap-s (access accp-entry entry :ap-s))
+         (ap-f (access accp-entry entry :ap-f))
+         (ap (+ ap-s ap-f))
+         (n-s (access accp-entry entry :n-s))
+         (n-f (access accp-entry entry :n-f))
+         (n (+ n-s n-f)))
+    (case key
+      ((:frames :frames-a) (list* ap ap-s n n-s lastcdr))
+      (:frames-s (list* ap-s ap n-s n lastcdr))
+      (:frames-f (list* ap-f ap n-f n lastcdr))
+      ((:tries :tries-a) (list* n n-s ap ap-s lastcdr))
+      (:tries-s (list* n-s n ap-s ap lastcdr))
+      (:tries-f  (list* n-f n ap-f ap lastcdr))
+      (:useless (list* ap n lastcdr))
+      (otherwise (list* (/ ap n) lastcdr)))))
+
+(defun show-accumulated-persistence-phrase2-merge (key alist last-key-info)
+
+; We augment the given alist by consing a sort key onto the front of each
+; entry.  The sort key is based on both the entry and the given key, the
+; first argument of show-accumulated-persistence.
+
   (cond ((null alist) nil)
-        (t (cons (cons (let* ((ap-s (access accp-entry (car alist) :ap-s))
-                              (ap-f (access accp-entry (car alist) :ap-f))
-                              (ap (+ ap-s ap-f))
-                              (n-s (access accp-entry (car alist) :n-s))
-                              (n-f (access accp-entry (car alist) :n-f))
-                              (n (+ n-s n-f)))
-                         (case key
-                           ((:frames :frames-a) (list* ap ap-s n n-s))
-                           (:frames-s (list* ap-s ap n-s n))
-                           (:frames-f (list* ap-f ap n-f n))
-                           ((:tries :tries-a) (list* n n-s ap ap-s))
-                           (:tries-s (list* n-s n ap-s ap))
-                           (:tries-f  (list* n-f n ap-f ap))
-                           (:useless (cons ap n))
-                           (otherwise (/ ap n))))
+        ((x-xrunep (access accp-entry (car alist) :xrune))
+         (cons (cons (append last-key-info
+                             (show-accumulated-persistence-phrase-key
+                              key
+                              (car alist)
+                              nil))
+                     (car alist))
+               (show-accumulated-persistence-phrase2-merge
+                key
+                (cdr alist)
+                last-key-info)))
+        (t (let ((next-key-info
+                  (show-accumulated-persistence-phrase-key
+                   key
+                   (car alist)
+                   (list (access accp-entry (car alist) :xrune)))))
+             (cons (cons (append next-key-info '(t))
+                         (car alist))
+                   (show-accumulated-persistence-phrase2-merge
+                    key
+                    (cdr alist)
+                    next-key-info))))))
+
+(defun show-accumulated-persistence-phrase2-not-merge (key alist)
+  (cond ((null alist) nil)
+        (t (cons (cons (show-accumulated-persistence-phrase-key key
+                                                                (car alist)
+                                                                nil)
                        (car alist))
-                 (show-accumulated-persistence-phrase2 key (cdr alist))))))
+                 (show-accumulated-persistence-phrase2-not-merge
+                  key (cdr alist))))))
+
+(defun show-accumulated-persistence-phrase2 (key alist mergep)
+  (cond (mergep (show-accumulated-persistence-phrase2-merge key alist nil))
+        (t (show-accumulated-persistence-phrase2-not-merge key alist))))
+
+(defun split-xrune-alist (alist rune-alist hyp-xrune-alist conc-xrune-alist)
+
+; See sort-rune-alist-for-xrunes.
+
+  (cond ((endp alist)
+         (mv rune-alist hyp-xrune-alist conc-xrune-alist))
+        (t (let ((xrune (access accp-entry (car alist) :xrune)))
+             (case (car xrune)
+               (:hyp  (split-xrune-alist (cdr alist)
+                                         rune-alist
+                                         (cons (car alist) hyp-xrune-alist)
+                                         conc-xrune-alist))
+               (:conc (split-xrune-alist (cdr alist)
+                                         rune-alist
+                                         hyp-xrune-alist
+                                         (cons (car alist) conc-xrune-alist)))
+               (t     (split-xrune-alist (cdr alist)
+                                         (cons (car alist) rune-alist)
+                                         hyp-xrune-alist
+                                         conc-xrune-alist)))))))
+
+(defun sort-xrune-alist-by-rune1 (rune-alist hyp-xrune-alist conc-xrune-alist
+                                             acc)
+
+; Each input alist is a list of accp-entry records, sorted by lexorder --
+; indeed sorted by the cars, which are distinct xrunes.  See
+; sort-rune-alist-for-xrunes.  We return the (disjoint) union of the three
+; inputs, such that every record for a :hyp or :conc xrune is preceded by an
+; entry whose :xrune is either another such xrune or is the corresponding rune.
+
+  (cond ((endp rune-alist)
+         (assert$ (and (null hyp-xrune-alist)
+                       (null conc-xrune-alist))
+                  acc))
+        ((and hyp-xrune-alist
+              (equal (hyp-xrune-rune (caar hyp-xrune-alist))
+                     (caar rune-alist)))
+         (sort-xrune-alist-by-rune1 rune-alist
+                                    (cdr hyp-xrune-alist)
+                                    conc-xrune-alist
+                                    (cons (car hyp-xrune-alist) acc)))
+        ((and conc-xrune-alist
+              (equal (conc-xrune-rune (caar conc-xrune-alist))
+                     (caar rune-alist)))
+         (sort-xrune-alist-by-rune1 rune-alist
+                                    hyp-xrune-alist
+                                    (cdr conc-xrune-alist)
+                                    (cons (car conc-xrune-alist) acc)))
+        (t
+         (sort-xrune-alist-by-rune1 (cdr rune-alist)
+                                    hyp-xrune-alist
+                                    conc-xrune-alist
+                                    (cons (car rune-alist) acc)))))
+
+(defun sort-xrune-alist-by-rune (alist display)
+
+; Alist is a list of accp-entry records.  We sort them such that every record
+; for a :hyp or :conc xrune is preceded either by an entry whose :xrune is
+; either another such xrune or is the corresponding rune.
+
+  (cond ((not (member-eq display '(nil :merge)))
+         alist)
+        (t (mv-let (rune-alist hyp-xrune-alist conc-xrune-alist)
+                   (split-xrune-alist alist nil nil nil)
+                   (cond ((eq display nil) rune-alist)
+                         (t ; (eq display :merge)
+                          (sort-xrune-alist-by-rune1
+                           (merge-sort-lexorder rune-alist)
+                           (merge-sort-lexorder hyp-xrune-alist)
+                           (merge-sort-lexorder conc-xrune-alist)
+                           nil)))))))
 
 (defun pop-accp-fn (info success-p)
 
-; Warning: Keep the two branches below in sync.
+; Warning: Keep the branches below in sync.  We considered merging them into a
+; single branch, but the fields changed differ in each case, so we keep the
+; cases separate in order to save a few conses.
 
-  (let ((rune-stack (access accp-info info :rune-stack)))
-    (if success-p
-        (let ((new-cnt (1+ (access accp-info info :cnt-s))))
-          (change accp-info info
-                  :cnt-s new-cnt
-                  :stack-s (cdr (access accp-info info :stack-s))
-                  :stack-f (cdr (access accp-info info :stack-f))
-                  :rune-stack (cdr rune-stack)
-                  :totals (add-accumulated-persistence
-                           (car rune-stack)
-                           success-p
-                           (- new-cnt
-                              (car (access accp-info info :stack-s)))
-                           (- (access accp-info info :cnt-f)
-                              (car (access accp-info info :stack-f)))
-                           (access accp-info info :totals))))
-      (let ((new-cnt (1+ (access accp-info info :cnt-f))))
-        (change accp-info info
-                :cnt-f new-cnt
-                :stack-s (cdr (access accp-info info :stack-s))
-                :stack-f (cdr (access accp-info info :stack-f))
-                :rune-stack (cdr rune-stack)
-                :totals (add-accumulated-persistence
-                         (car rune-stack)
-                         success-p
-                         (- (access accp-info info :cnt-s)
-                            (car (access accp-info info :stack-s)))
-                         (- new-cnt
-                            (car (access accp-info info :stack-f)))
-                         (access accp-info info :totals)))))))
+  (let* ((xrune-stack (access accp-info info :xrune-stack))
+         (xrune (car xrune-stack))
+         (xp (x-xrunep xrune))
+         (new-cnt (and (not xp) ; optimization
+                       (cond (success-p
+                              (1+ (access accp-info info :cnt-s)))
+                             (t
+                              (1+ (access accp-info info :cnt-f)))))))
+    (cond
+     (xp
+      (change accp-info info
+              :stack-s (cdr (access accp-info info :stack-s))
+              :stack-f (cdr (access accp-info info :stack-f))
+              :xrune-stack (cdr xrune-stack)
+              :totals (add-accumulated-persistence
+                       xrune
+                       success-p
+                       (- (access accp-info info :cnt-s)
+                          (car (access accp-info info :stack-s)))
+                       (- (access accp-info info :cnt-f)
+                          (car (access accp-info info :stack-f)))
+                       (access accp-info info :totals))))
+     (success-p
+      (change accp-info info
+              :cnt-s new-cnt
+              :stack-s (cdr (access accp-info info :stack-s))
+              :stack-f (cdr (access accp-info info :stack-f))
+              :xrune-stack (cdr xrune-stack)
+              :totals (add-accumulated-persistence
+                       xrune
+                       success-p
+                       (- new-cnt
+                          (car (access accp-info info :stack-s)))
+                       (- (access accp-info info :cnt-f)
+                          (car (access accp-info info :stack-f)))
+                       (access accp-info info :totals))))
+     (t
+      (change accp-info info
+              :cnt-f new-cnt
+              :stack-s (cdr (access accp-info info :stack-s))
+              :stack-f (cdr (access accp-info info :stack-f))
+              :xrune-stack (cdr xrune-stack)
+              :totals (add-accumulated-persistence
+                       xrune
+                       success-p
+                       (- (access accp-info info :cnt-s)
+                          (car (access accp-info info :stack-s)))
+                       (- new-cnt
+                          (car (access accp-info info :stack-f)))
+                       (access accp-info info :totals)))))))
 
 (defun pop-accp-fn-iterate (info n)
   (if (zp n)
@@ -6292,18 +6809,20 @@ gbc time        :      8.930 secs
                                       t)
                          (1- n))))
 
-(defun show-accumulated-persistence-phrase (key accp-info)
+(defun show-accumulated-persistence-phrase (key/display accp-info)
 
 ; Alist is the accumulated totals alist from the wormhole data field of
 ; wormhole-status of the 'accumulated-persistence wormhole.  Each element is of
-; the form (rune n . ap) and we sort them into descending order on the
+; the form (xrune n . ap) and we sort them into descending order on the
 ; specified key.  Key should be one of the sortkey values from the guard of
 ; show-accumulated-persistence.
 
-  (let* ((rune-stack (access accp-info accp-info :rune-stack))
-         (accp-info (cond ((and rune-stack
+  (let* ((key (car key/display))
+         (display (cdr key/display))
+         (xrune-stack (access accp-info accp-info :xrune-stack))
+         (accp-info (cond ((and xrune-stack
                                 (member-eq key '(:frames-a :tries-a)))
-                           (pop-accp-fn-iterate accp-info (length rune-stack)))
+                           (pop-accp-fn-iterate accp-info (length xrune-stack)))
                           (t accp-info)))
          (totals (access accp-info accp-info :totals)))
     (cond
@@ -6311,25 +6830,33 @@ gbc time        :      8.930 secs
       (msg "There is no accumulated persistence to show.  Evaluate ~x0 to ~
             activate gathering of accumulated-persistence statistics.~|"
            '(accumulated-persistence t)))
-     (t (let ((main-phrase
-               (list "" "~@*" "~@*" "~@*" 
-                     (show-accumulated-persistence-phrase1
-                      key
-                      (merge-sort-lexorder
+     (t (let* ((mergep (eq display :merge))
+               (alist (merge-sort-lexorder
                        (show-accumulated-persistence-phrase2
-                        key (car (last totals))))
-                      nil))))
+                        key
+                        (sort-xrune-alist-by-rune (car (last totals))
+                                                  display)
+                        mergep)))
+               (main-phrase
+                (list "" "~@*" "~@*" "~@*" 
+                      (show-accumulated-persistence-phrase1
+                       key
+                       (if (eq key :useless)
+                           (show-accumulated-persistence-remove-useless alist
+                                                                        nil)
+                         alist)
+                       mergep
+                       nil))))
           (cond ((null (cdr totals))
                  (msg "Accumulated Persistence~@0~|~%   :frames   :tries    ~
-                       :ratio  rune~%~@1~*2"
-                      (if (and rune-stack
-                               (null (cdr totals)))
+                       :ratio  rune~%~*1~@2"
+                      (if xrune-stack
                           "" ; we merged, so don't know just what was useful
                         (msg " (~x0 :tries useful, ~x1 :tries not useful)"
                              (access accp-info accp-info :cnt-s)
                              (access accp-info accp-info :cnt-f)))
-                      *accp-separator*
-                      main-phrase))
+                      main-phrase
+                      *accp-major-separator*))
                 (t
                  (msg "Accumulated Persistence~|~%~
                        ***************************************~|~
@@ -6338,24 +6865,30 @@ gbc time        :      8.930 secs
                        *** Use :frames-a or :tries-a to get more complete ~
                            totals.~|~
                        ***************************************~|~
-                       ~%   :frames   :tries    :ratio  rune~%~@1~*2"
+                       ~%   :frames   :tries    :ratio  rune~%~*1~@2"
                       (- (+ (access accp-info accp-info
                                     :cnt-s)
                             (access accp-info accp-info
                                     :cnt-f)
-                            (length rune-stack))
+                            (length xrune-stack))
                          (+ (car (last (access accp-info accp-info
                                                :stack-s)))
                             (car (last (access accp-info accp-info
                                                :stack-f)))))
-                      *accp-separator*
-                      main-phrase))))))))
+                      main-phrase
+                      *accp-major-separator*))))))))
 
-(defmacro show-accumulated-persistence (&optional (sortkey ':frames))
-  (declare (xargs :guard (member-eq sortkey '(:ratio
-                                              :frames :frames-s :frames-f :frames-a
-                                              :tries :tries-s :tries-f :tries-a
-                                              :useless))))
+(defmacro show-accumulated-persistence (&optional (sortkey ':frames)
+                                                  (display 't))
+  (declare (xargs :guard
+                  (and (member-eq sortkey
+                                  '(:ratio
+                                    :frames :frames-s :frames-f :frames-a
+                                    :tries :tries-s :tries-f :tries-a
+                                    :useless))
+                       (member-eq display
+                                  '(t nil :raw :merge)))))
+
 ; This function engages is in a little song-and-dance about the entry code for
 ; the accumulated-persistence wormhole.  If the user has requested that we
 ; print the accumulated-persistence data, we enter the wormhole to do it --
@@ -6367,11 +6900,10 @@ gbc time        :      8.930 secs
 ; code was :SKIP, the data was nil anyway.  Once inside, if the data is
 ; :RETURN-TO-SKIP we set the entry code back to :SKIP.
 
-
   `(wormhole 'accumulated-persistence
              '(lambda (whs)
                 (set-wormhole-entry-code whs :ENTER))
-             ,sortkey
+             ',(cons sortkey display)
              '(pprogn
                (io? temporary nil state
                     nil
@@ -6394,7 +6926,7 @@ gbc time        :      8.930 secs
              :ld-query-control-alist nil
              :ld-verbose nil))
 
-(defun push-accp (rune)
+(defun push-accp (rune x-info)
   (wormhole-eval 'accumulated-persistence
                  '(lambda (whs)
 
@@ -6407,54 +6939,74 @@ gbc time        :      8.930 secs
 ; be a accp-info record.  See the Essay on Wormholes.
 
                     (let ((info (wormhole-data whs)))
-                      (if info
-                          (set-wormhole-data
-                           whs
-                           (change accp-info info
-                                   :rune-stack (cons rune (access accp-info info :rune-stack))
-                                   :stack-s (cons (access accp-info info :cnt-s)
-                                                  (access accp-info info :stack-s))
-                                   :stack-f (cons (access accp-info info :cnt-f)
-                                                  (access accp-info info :stack-f))
-                                   :totals (cons nil
-                                                 (access accp-info info :totals))))
+                      (if (and info
+                               (or (null x-info)
+                                   (access accp-info info :xrunep)))
+                          (let ((xrune (cond ((natp x-info)
+                                              (hyp-xrune x-info rune))
+                                             ((eq x-info :conc)
+                                              (conc-xrune rune))
+                                             ((null x-info)
+                                              rune)
+                                             (t (er hard 'push-accp
+                                                    "Implementation error: ~
+                                                     Bad value of x-info, ~x0."
+                                                    x-info)))))
+                            (set-wormhole-data
+                             whs
+                             (change accp-info info
+                                     :xrune-stack (cons xrune (access accp-info
+                                                                      info
+                                                                      :xrune-stack))
+                                     :stack-s (cons (access accp-info info :cnt-s)
+                                                    (access accp-info info :stack-s))
+                                     :stack-f (cons (access accp-info info :cnt-f)
+                                                    (access accp-info info :stack-f))
+                                     :totals (cons nil
+                                                   (access accp-info info :totals)))))
                           whs)))
                  rune))
 
-(defun pop-accp (success-p)
+(defun pop-accp (success-p x-info)
   (wormhole-eval 'accumulated-persistence
                  '(lambda (whs)
                     (let ((info (wormhole-data whs)))
-                      (if info
+                      (if (and info
+                               (or (null x-info)
+                                   (access accp-info info :xrunep)))
                           (set-wormhole-data whs
                                              (pop-accp-fn info success-p))
                           whs)))
                  success-p))
 
-(defmacro with-accumulated-persistence (rune vars success-p body)
-  `(let ((with-accumulated-persistence-rune ,rune))
-     (prog2$
-      (push-accp with-accumulated-persistence-rune)
-      ,(cond ((and (true-listp vars)
-                   (= (length vars) 1))
-              `(let ((,(car vars)
-                      (check-vars-not-free
-                       (with-accumulated-persistence-rune)
-                       ,body)))
-                 (prog2$
-                  (pop-accp (check-vars-not-free
-                             (with-accumulated-persistence-rune)
-                             ,success-p))
-                  ,(car vars))))
-             (t `(mv-let ,vars
-                         (check-vars-not-free
-                          (with-accumulated-persistence-rune)
-                          ,body)
-                         (prog2$
-                          (pop-accp (check-vars-not-free
-                                     (with-accumulated-persistence-rune)
-                                     ,success-p))
-                          (mv ,@vars))))))))
+(defmacro with-accumulated-persistence (rune vars success-p body
+                                             &optional
+                                             x-info
+                                             (condition 'nil condition-p))
+
+; X-info can be :conc to indicate that we are tracking the right-hand side of a
+; rule, or a positive integer n to indicate that we are tracking the nth
+; hypothesis of a rule.  Otherwise x-info should be nil.
+
+  (let ((form
+         `(prog2$
+           (push-accp ,rune ,x-info)
+           ,(cond ((and (true-listp vars)
+                        (= (length vars) 1))
+                   `(let ((,(car vars)
+                           ,body))
+                      (prog2$
+                       (pop-accp ,success-p ,x-info)
+                       ,(car vars))))
+                  (t `(mv-let ,vars
+                              ,body
+                              (prog2$
+                               (pop-accp ,success-p ,x-info)
+                               (mv ,@vars))))))))
+    (cond (condition-p
+           `(cond (,condition ,form)
+                  (t ,body)))
+          (t form))))
 
 ;; RAG - Changed the assumptions based on rational to realp.
 
@@ -7331,7 +7883,7 @@ gbc time        :      8.930 secs
         (t 
 
 ; Otherwise, we apply all known type-prescriptions and conclude with
-; whatever is builtin about fn.
+; whatever is built in about fn.
 
 ; Note: We do not know that 'type-prescriptions is non-nil.  Once upon
 ; a time we insisted that every fn have a type-prescription.  This
@@ -7378,7 +7930,7 @@ gbc time        :      8.930 secs
 (defun type-set-relieve-hyps (rune target hyps backchain-limit-lst
                                    force-flg dwp alist type-alist
                                    ancestors ens wrld ttree ttree0 pot-lst pt
-                                   backchain-limit)
+                                   backchain-limit bkptr)
 
 ; Hyps is a list of terms, implicitly conjoined.  Alist is a substitution
 ; mapping variables in hyps to terms governed by type-alist.  Consider the
@@ -7407,7 +7959,7 @@ gbc time        :      8.930 secs
             force-flg dwp
             (cons (cons (fargn hyp 1) (fargn hyp 2)) alist)
             type-alist ancestors ens wrld ttree ttree0
-            pot-lst pt backchain-limit))
+            pot-lst pt backchain-limit (1+ bkptr)))
           (t
            (mv-let
             (lookup-hyp-ans alist ttree)
@@ -7421,8 +7973,22 @@ gbc time        :      8.930 secs
                                      force-flg dwp alist
                                      type-alist ancestors ens wrld
                                      ttree ttree0
-                                     pot-lst pt backchain-limit))
+                                     pot-lst pt backchain-limit (1+ bkptr)))
              ((free-varsp hyp alist)
+              (let ((fully-bound-alist
+                     (if (and forcep force-flg)
+                         (bind-free-vars-to-unbound-free-vars
+                          (all-vars hyp)
+                          alist)
+                         alist)))
+
+; Fully-bound-alist is an extension of alist in which all vars occurring
+; in hyp are bound to something.  A var v that occurs freely in hyp wrt
+; alist is bound in fully-bound-alist to UNBOUND-FREE-v.  But we only
+; compute the all-vars and fully-bound-alist if we're going to use it
+; below.  For sanity, fully-bound-alist is just alist if we're not
+; actually intending to use it.
+
               (mv-let
                (force-flg ttree)
                (cond
@@ -7431,21 +7997,26 @@ gbc time        :      8.930 secs
                 (t (force-assumption
                     rune
                     target
-                    (sublis-var-and-mark-free alist hyp)
+                    (sublis-var fully-bound-alist hyp)
                     type-alist
                     nil
                     (immediate-forcep (ffn-symb (car hyps)) ens)
                     force-flg
                     ttree)))
+
+; Note that force-flg has been rebound by the mv-let above.  Think of
+; it as just a temporary variable meaning (and forcep force-flg) and
+; we use it only if it is true.
+ 
                (cond
                 (force-flg
                  (type-set-relieve-hyps
                   rune target (cdr hyps) (cdr backchain-limit-lst)
                   force-flg dwp
-                  alist type-alist ancestors ens wrld
+                  fully-bound-alist type-alist ancestors ens wrld
                   ttree ttree0
-                  pot-lst pt backchain-limit))
-                (t (mv nil type-alist ttree0)))))
+                  pot-lst pt backchain-limit (1+ bkptr)))
+                (t (mv nil type-alist ttree0))))))
              (t
               (mv-let
                (not-flg atm)
@@ -7473,7 +8044,8 @@ gbc time        :      8.930 secs
                                                 force-flg dwp alist
                                                 type-alist ancestors ens wrld
                                                 ttree ttree0
-                                                pot-lst pt backchain-limit))
+                                                pot-lst pt backchain-limit
+                                                (1+ bkptr)))
                         (t (mv nil type-alist ttree0))))
                  (t
                   (mv-let
@@ -7500,7 +8072,8 @@ gbc time        :      8.930 secs
                                               force-flg dwp alist
                                               type-alist ancestors ens wrld
                                               ttree ttree0
-                                              pot-lst pt backchain-limit))
+                                              pot-lst pt backchain-limit
+                                              (1+ bkptr)))
                       (t (mv nil type-alist ttree0))))
                     ((backchain-limit-reachedp backchain-limit ancestors)
                      (mv-let
@@ -7529,86 +8102,73 @@ gbc time        :      8.930 secs
                          (cdr backchain-limit-lst)
                          force-flg dwp alist type-alist ancestors
                          ens wrld ttree ttree0 pot-lst pt
-                         backchain-limit))
+                         backchain-limit (1+ bkptr)))
                        (t (mv nil type-alist ttree0)))))
-                    (t 
+                    (t
                      (mv-let
-                      (ts1 ttree1)
-                      (type-set-rec atm1 force-flg dwp type-alist
+                      (flg type-alist ttree2)
+                      (with-accumulated-persistence
+                       rune
+                       (flg type-alist ttree2)
+                       flg
+                       (mv-let
+                        (ts1 ttree1)
+                        (type-set-rec atm1 force-flg dwp type-alist
 
 ; We know ancestors is not t here, by the tests above.
 
-                                    (push-ancestor
-                                     (if not-flg
-                                         atm1
-                                       (mcons-term* 'not atm1))
-                                     (list rune)
-                                     ancestors)
-                                    ens wrld ttree
-                                    pot-lst pt
-                                    (new-backchain-limit
-                                     (car backchain-limit-lst)
-                                     backchain-limit
-                                     ancestors))
-                      (mv-let (temp1 temp2)
-                              (assoc-type-alist atm1 type-alist wrld)
-                              (declare (ignore temp2))
-                              (let ((type-alist
-                                     (cond ((and temp1 (ts-subsetp temp1 ts1))
-                                            type-alist)
-                                           (t (extend-type-alist
-                                               ;;*** -simple
-                                               atm1 ts1 ttree1 type-alist
-                                               wrld))))
-                                    (ts (if not-flg
-                                            (cond ((ts= ts1 *ts-nil*) *ts-t*)
-                                                  ((ts-intersectp ts1 *ts-nil*)
-                                                   *ts-boolean*)
-                                                  (t *ts-nil*))
-                                          ts1)))
-                                (cond
-                                 ((ts= ts *ts-nil*) (mv nil type-alist ttree0))
-                                 ((ts-intersectp *ts-nil* ts)
-                                  (mv-let
-                                   (force-flg ttree)
-                                   (cond
-                                    ((not (and force-flg forcep))
-                                     (mv nil ttree))
-                                    (t (force-assumption
-                                        rune
-                                        target
-                                        (if not-flg
-                                            (mcons-term* 'not atm1)
-                                          atm1)
-                                        type-alist nil
-                                        (immediate-forcep
-                                         (ffn-symb (car hyps))
-                                         ens)
-                                        force-flg
-                                        ttree1)))
-                                   (cond
-                                    (force-flg
-                                     (type-set-relieve-hyps
-                                      rune
-                                      target
-                                      (cdr hyps)
-                                      (cdr backchain-limit-lst)
-                                      force-flg dwp alist type-alist ancestors
-                                      ens wrld ttree ttree0 pot-lst pt
-                                      backchain-limit))
-                                    (t (mv nil type-alist ttree0)))))
-                                 (t (type-set-relieve-hyps
-                                     rune
-                                     target
-                                     (cdr hyps)
-                                     (cdr backchain-limit-lst)
-                                     force-flg dwp alist
-                                     type-alist ancestors
-                                     ens wrld
-                                     ttree1 ttree0
-                                     pot-lst
-                                     pt
-                                     backchain-limit)))))))))))))))))))))))
+                                      (push-ancestor
+                                       (if not-flg
+                                           atm1
+                                         (mcons-term* 'not atm1))
+                                       (list rune)
+                                       ancestors)
+                                      ens wrld ttree
+                                      pot-lst pt
+                                      (new-backchain-limit
+                                       (car backchain-limit-lst)
+                                       backchain-limit
+                                       ancestors))
+                        (let ((ts (if not-flg
+                                      (cond ((ts= ts1 *ts-nil*) *ts-t*)
+                                            ((ts-intersectp ts1 *ts-nil*)
+                                             *ts-boolean*)
+                                            (t *ts-nil*))
+                                    ts1)))
+                          (cond
+                           ((ts= ts *ts-nil*) (mv nil type-alist ttree0))
+                           ((ts-intersectp *ts-nil* ts)
+                            (mv-let
+                             (force-flg ttree)
+                             (cond
+                              ((not (and force-flg forcep))
+                               (mv nil ttree))
+                              (t (force-assumption
+                                  rune
+                                  target
+                                  (if not-flg
+                                      (mcons-term* 'not atm1)
+                                    atm1)
+                                  type-alist nil
+                                  (immediate-forcep
+                                   (ffn-symb (car hyps))
+                                   ens)
+                                  force-flg
+                                  ttree)))
+                             (cond
+                              (force-flg (mv t type-alist ttree))
+                              (t (mv nil type-alist ttree0)))))
+                           (t (mv t type-alist ttree1)))))
+                       bkptr)
+                      (cond (flg (type-set-relieve-hyps
+                                  rune
+                                  target
+                                  (cdr hyps)
+                                  (cdr backchain-limit-lst)
+                                  force-flg dwp alist type-alist ancestors
+                                  ens wrld ttree2 ttree0 pot-lst pt
+                                  backchain-limit (1+ bkptr)))
+                            (t (mv nil type-alist ttree2)))))))))))))))))))))
 
 (defun extend-type-alist-with-bindings (alist force-flg dwp type-alist
                                               ancestors ens w ttree pot-lst pt
@@ -7701,19 +8261,25 @@ gbc time        :      8.930 secs
 
                                   nil
                                   ttree
-                                  pot-lst pt backchain-limit)
+                                  pot-lst pt backchain-limit 1)
            (cond
             (relieve-hyps-ans
-             (type-set-with-rule1 unify-subst
-                                  (access type-prescription tp :vars)
-                                  force-flg
-                                  dwp
-                                  type-alist ancestors ens w
-                                  (access type-prescription tp :basic-ts)
-                                  (push-lemma
-                                   (access type-prescription tp :rune)
-                                   ttree)
-                                  pot-lst pt backchain-limit))
+             (with-accumulated-persistence
+              (access type-prescription tp :rune)
+              (ts type-alist ttree)
+              (ts= ts *ts-unknown*)
+              (type-set-with-rule1 unify-subst
+                                   (access type-prescription tp :vars)
+                                   force-flg
+                                   dwp
+                                   type-alist ancestors ens w
+                                   (access type-prescription tp :basic-ts)
+                                   (push-lemma
+                                    (access type-prescription tp :rune)
+                                    ttree)
+                                   pot-lst pt backchain-limit)
+              :conc
+              hyps))
             (t (mv *ts-unknown* type-alist ttree)))))))
       (t (mv *ts-unknown* type-alist ttree)))))
    (t (mv *ts-unknown* type-alist ttree))))
@@ -9216,7 +9782,7 @@ gbc time        :      8.930 secs
 ; In the mv-let below we effectively implement the facts that, when x
 ; is of type *ts-integer* (< x 1) is ~(< 0 x), and (< -1 x) is ~(< x
 ; 0).  By normalizing such inequalities around 0 we can more easily
-; recognize the ones covered by our builtin types.
+; recognize the ones covered by our built in types.
 
 ; WARNING: A bug once lurked here, so beware.  The term we are
 ; assuming is represented by xnot-flg and x.  We are about to
